%%%%%%%%%%%%%%%%%%%%%%%%%%%%%%%%%%%%%%%%%%%%%%%%%%%%%%%%%%%%%%%%%%%%%%%%%%%%%%%%%%%%%%%%%%%%%%%%%%%%%%%%%%%%%%%%%%%%%%%%%%%%%%%%%%%%%%%%%%%%%%%%%%%%%%%%%%%%%%%%%%%
% Written By Michael Brodskiy
% Class: Quantum Mechanics
% Professor: G. Fiete
%%%%%%%%%%%%%%%%%%%%%%%%%%%%%%%%%%%%%%%%%%%%%%%%%%%%%%%%%%%%%%%%%%%%%%%%%%%%%%%%%%%%%%%%%%%%%%%%%%%%%%%%%%%%%%%%%%%%%%%%%%%%%%%%%%%%%%%%%%%%%%%%%%%%%%%%%%%%%%%%%%%

\include{Includes.tex}

\title{Homework 3}
\date{\today}
\author{Michael Brodskiy\\ \small Professor: G. Fiete}

\begin{document}

\maketitle

\begin{enumerate}

  \item

    \begin{enumerate}

      \item We know that, for a spin-1 system, the spin can be:

        $$\boxed{S_z=\hbar,0,-\hbar}$$

        Given the quantum state in the problem, we can find the probabilities of each as:

        $$P_1=\left( \frac{1}{\sqrt{30}} \right)^2$$
        $$P_0=\left( \frac{2}{\sqrt{30}} \right)^2$$
        $$P_{-1}=\left( \frac{|5i|}{\sqrt{30}} \right)^2$$

        This gives us:

        $$\boxed{\left\{\begin{array}{ll} P_1&= 1/30\\P_0&= 2/15\\P_{-1}&= 5/6\end{array}}$$

          We can calculate the expectation value of $S_z$ by using:

          $$\bra{\psi|S_z}\ket{\psi}$$

          In matrix notation, this gives us:

          $$<S_z>=\left[ \frac{\hbar}{30} \right](1\quad 2\quad -5i)\left( \begin{matrix} 1 & 0 & 0\\ 0 & 0 & 0\\ 0 & 0 & -1\end{matrix} \right)\left( \begin{matrix}1\\2\\5i\end{matrix} \right)$$

          We proceed to evaluate:

          $$<S_z>=\left[ \frac{\hbar}{30} \right](1\quad 0\quad 5i)\left( \begin{matrix}1\\2\\5i\end{matrix} \right)$$
          $$<S_z>=\left[ \frac{\hbar}{30} \right](1-(25))$$
          $$\boxed{<S_z>= -\frac{24\hbar}{30}=-\frac{12\hbar}{15}}$$

        \item Similar to the expectation value of $S_z$ in part (a), we apply the matrix notation of $S_x$ to write:

          $$<S_x>=\left[ \frac{\hbar}{30\sqrt{2}} \right](1\quad 2\quad -5i)\left( \begin{matrix} 0 & 1 & 0\\ 1 & 0 & 1\\ 0 & 1 & 0\end{matrix} \right)\left( \begin{matrix}1\\2\\5i\end{matrix} \right)$$
          $$<S_x>=\left[ \frac{\hbar}{30\sqrt{2}} \right](2\quad 1-5i\quad 2)\left( \begin{matrix}1\\2\\5i\end{matrix} \right)$$
          $$<S_x>=\left[ \frac{\hbar}{30\sqrt{2}} \right](4+10i-10i)$$
          $$\boxed{<S_x>= \frac{4\hbar}{30\sqrt{2}}=\frac{2\hbar}{15\sqrt{2}}}$$

    \end{enumerate}

  \item We may begin by converting $\ket{\psi_f}$ into the $S_z$ basis to simply probability calculations. We know:

    $$\ket{1}=\frac{1}{2}\left( \ket{1}+i\sqrt{2}\ket{0}-\ket{-1} \right)$$
    $$\ket{0}=\frac{1}{\sqrt{2}}\left( \ket{1}+\ket{-1} \right)$$
    $$\ket{-1}=\frac{1}{2}\left( \ket{1}-i\sqrt{2}\ket{0}-\ket{-1} \right)$$

    Applying this to the given state function, we may find:

    $$\ket{\psi_f}=\frac{1+i}{2\sqrt{7}}\left[ \ket{1}+i\sqrt{2}\ket{0}-\ket{-1}\right]+\frac{2}{\sqrt{14}}\left[\ket{1}+\ket{-1} \right]-\frac{i}{2\sqrt{7}}\left[ \ket{1}-i\sqrt{2}\ket{0}-\ket{-1}\right]$$

    We distribute and simplify:

    $$\ket{\psi_f}=\left[\frac{1+i}{2\sqrt{7}}+\frac{2}{\sqrt{14}}-\frac{i}{2\sqrt{7}}\right]\ket{1}+\left[\frac{i-1}{\sqrt{14}}-\frac{1}{\sqrt{14}}\right]\ket{0}+\left[-\frac{1+i}{2\sqrt{7}}+\frac{2}{\sqrt{14}}+\frac{i}{2\sqrt{7}}\right]\ket{-1}$$
    $$\ket{\psi_f}=\left[\frac{1}{2\sqrt{7}}+\frac{\sqrt{2}}{\sqrt{7}}\right]\ket{1}+\left[\frac{i-2}{\sqrt{14}}\right]\ket{0}+\left[-\frac{1}{2\sqrt{7}}+\frac{\sqrt{2}}{\sqrt{7}}\right]\ket{-1}$$
    $$\ket{\psi_f}=\left[\frac{1+2\sqrt{2}}{2\sqrt{7}}\right]\ket{1}+\left[\frac{i-2}{\sqrt{14}}\right]\ket{0}+\left[\frac{2\sqrt{2}-1}{2\sqrt{7}}\right]\ket{-1}$$

    We know that the probability of a normalized state (like $\psi_i$) can be expressed as:

    $$P=|\bra{\psi_f}\ket{\psi_i}|^2$$

    We take the complex conjugate to get:

    $$\bra{\psi_f}=\left[\frac{1+2\sqrt{2}}{2\sqrt{7}}\right]\ket{1}-\left[\frac{i+2}{\sqrt{14}}\right]\ket{0}+\left[\frac{2\sqrt{2}-1}{2\sqrt{7}}\right]\ket{-1}$$

    We proceed to take the inner product of the two:

    $$\bra{\psi_f}\ket{\psi_i}=\left[ \frac{1+2\sqrt{2}}{2\sqrt{7}} \right]\left[ \sqrt{\frac{1}{6}} \right]+\left[ \frac{i+2}{\sqrt{14}} \right]\left[ \sqrt{\frac{2}{6}} \right]+\left[ \frac{2\sqrt{2}-1}{2\sqrt{7}} \right]\left[ i\sqrt{\frac{3}{6}} \right]$$

    We then simplify:

    $$\bra{\psi_f}\ket{\psi_i}=\frac{1+2\sqrt{2}}{2\sqrt{42}}+\frac{i+2}{\sqrt{42}}+\left[ \frac{1}{\sqrt{7}}-\frac{1}{2\sqrt{14}} \right]i$$
    
    For ease of calculation, we may convert to decimal form:

    $$\bra{\psi_f}\ket{\psi_i}=.604+.3986i$$

    We can then find the probability as:

    $$|\bra{\psi_f}\ket{\psi_i}|^2=.604^2+.3986^2$$
    $$\boxed{P=.5237}$$

  \item

    \begin{enumerate}

      \item We know that $\hat{A}$ and $\hat{B}$ commute if $\hat{A}\hat{B}=\hat{B}\hat{A}$. Thus, we begin by calculating $\hat{A}\hat{B}$:

        $$\hat{A}\hat{B}=\left( \begin{matrix} a_1 & 0 & 0\\ 0 & a_2 & 0\\ 0 & 0 & a_3\end{matrix} \right)\left( \begin{matrix} b_1 & 0 & 0\\ 0 & 0 & b_2\\ 0 & b_2 & 0\end{matrix} \right)$$

        This gives us:

        $$\hat{A}\hat{B}=\left( \begin{matrix} a_1b_1 & 0 & 0\\ 0 & 0 & a_2b_2\\ 0 & a_3b_2 & 0\end{matrix} \right)$$

        Now, we calculate $\hat{B}\hat{A}$:

        $$\hat{B}\hat{A}=\left( \begin{matrix} b_1 & 0 & 0\\ 0 & 0 & b_2\\ 0 & b_2 & 0\end{matrix} \right)\left( \begin{matrix} a_1 & 0 & 0\\ 0 & a_2 & 0\\ 0 & 0 & a_3\end{matrix} \right)$$

        This gives us:

        $$\hat{B}\hat{A}=\left( \begin{matrix} b_1a_1 & 0 & 0\\ 0 & 0 & b_2a_3\\ 0 & b_2a_2&0\end{matrix} \right)$$

        We may see that $\hat{A}\hat{B}\neq\hat{B}\hat{A}$ and, therefore, the operators \underline{do not commute}

      \item We begin working with $\hat{A}$:

        $$|\hat{A}-\lambda\mathbb{1}|=0$$

        This gives us:

        $$(a_1-\lambda)(a_2-\lambda)(a_3-\lambda)=0$$

        Thus, we see that, since this is a diagonal matrix, we get $\boxed{\lambda=a_1, a_2,\text{ and }a_3}$ as the eigenvalues. Thus, we may observe that the normalized eigenvectors are:

        $$\boxed{\left\{ \left[ \begin{matrix} 1\\0\\0\end{matrix} \right], \left[ \begin{matrix}0\\1\\0\end{matrix} \right],\left[ \begin{matrix} 0\\0\\1\end{matrix} \right] \right\}}$$

        We then proceed to do the same with $\hat{B}$:

        $$\Big|\left[ \begin{matrix} b_1-\lambda & 0 & 0\\ 0 & -\lambda & b_2\\0 & b_2 & -\lambda\end{matrix} \right]\Big|=0$$

        This gives us:

        $$(b_1-\lambda)(\lambda^2-b_2^2)=0$$

        We can thus see that the eigenvalues are:

        $$\boxed{\lambda=b_1,\pm b_2}$$

        From here, we can observe that the normalized eigenvectors become:

        $$\boxed{\left[ \begin{matrix} 1 \\ 0 \\ 0 \end{matrix}\right],\frac{1}{\sqrt{2}}\left[ \begin{matrix} 0\\1\\1\end{matrix} \right],\frac{1}{\sqrt{2}}\left[ \begin{matrix}0\\-1\\1\end{matrix} \right]}$$

      \item Let us assume that the basis eigenvectors are:

        $$\ket{1}= \left[ \begin{matrix} 1\\0\\0\end{matrix} \right],\quad\ket{2}=\left[ \begin{matrix}0\\1\\0\end{matrix} \right],\ket{3}=\left[ \begin{matrix} 0\\0\\1\end{matrix} \right]$$

        We calculate the measure of $\hat{B}$ by writing:

        $$\hat{B}\ket{2}=\left( \begin{matrix} b_1 & 0 & 0\\ 0 & 0 & b_2\\ 0 & b_2 & 0\end{matrix} \right)\left( \begin{matrix}0\\1\\0\end{matrix} \right)$$
        $$\hat{B}\ket{2}=\left( \begin{matrix}0\\0\\b_2\end{matrix} \right)$$

        Rewriting this in terms of the basis vectors of $\hat{B}$, we may find:

        $$\hat{B}\ket{2}=\frac{b_2}{2}\left(\left[ \begin{matrix} 0\\1\\1\end{matrix} \right]+\left[ \begin{matrix}0\\-1\\1\end{matrix} \right]  \right)$$
        $$\boxed{\hat{B}\ket{2}=\frac{b_2}{\sqrt{2}}\left(\ket{B_2}+\ket{B_3}  \right)}$$

        Since we may see that the two occur with equal probabilities, we may say that, for the operator $\hat{B}$, the probabilities are $P_{B_2}=P_{B_3}=.5$, while $P_{B_1}=0$ (where $B_1$ corresponds to $b_1$, $B_2$ to $b_2$ and $B_3$ to $-b_2$ eigenvalue solutions)

        On the other hand, we may find the probabilities of subsequently measuring $a$ (after $\ket{2}$) to be:

        $$P_{\pm b_2,a_1}=|\bra{a_1}\ket{B_2}|^2\to |\bra{1}\frac{1}{\sqrt{2}}(\ket{2}\pm\ket{3})|^2$$
        $$P_{\pm b_2,a_2}=|\bra{a_2}\ket{B_2}|^2\to |\bra{2}\frac{1}{\sqrt{2}}(\ket{2}\pm\ket{3})|^2$$
        $$P_{\pm b_2,a_3}=|\bra{a_3}\ket{B_2}|^2\to |\bra{3}\frac{1}{\sqrt{2}}(\ket{2}\pm\ket{3})|^2$$

      Since we know that the inner product of the same basis vectors produces one and two different basis vectors produces zero due to orthonormality, we find:

        $$\boxed{P_{\pm b_2,a_1}=0}$$
        $$P_{\pm b_2,a_2}=\Big|\frac{\pm 1}{\sqrt{2}}\Big|^2$$
        $$P_{\pm b_2,a_3}=\Big|\frac{\pm 1}{\sqrt{2}}\Big|^2$$

        And finally:

        $$\boxed{P_{\pm b_2,a_2}=\frac{1}{2}}$$
        $$\boxed{P_{\pm b_2,a_3}=\frac{1}{2}}$$

        We may note that the sign on the $\ket{3}$ term is irrelevant, as we only care about the magnitude.

      \item Note that the result from part (a) indicates that we can not know the measurements of $A$ and $B$ at the same time with certainty. This is confirmed by the results from part (c), as we find that measuring $\hat{B}\ket{2}$ before $\hat{A}$ has no effect on the result of $\hat{A}$

    \end{enumerate}

\end{enumerate}

\end{document}

