%%%%%%%%%%%%%%%%%%%%%%%%%%%%%%%%%%%%%%%%%%%%%%%%%%%%%%%%%%%%%%%%%%%%%%%%%%%%%%%%%%%%%%%%%%%%%%%%%%%%%%%%%%%%%%%%%%%%%%%%%%%%%%%%%%%%%%%%%%%%%%%%%%%%%%%%%%%%%%%%%%%
% Written By Michael Brodskiy
% Class: Quantum Mechanics
% Professor: G. Fiete
%%%%%%%%%%%%%%%%%%%%%%%%%%%%%%%%%%%%%%%%%%%%%%%%%%%%%%%%%%%%%%%%%%%%%%%%%%%%%%%%%%%%%%%%%%%%%%%%%%%%%%%%%%%%%%%%%%%%%%%%%%%%%%%%%%%%%%%%%%%%%%%%%%%%%%%%%%%%%%%%%%%

\include{Includes.tex}

\title{Lecture 5}
\date{\today}
\author{Michael Brodskiy\\ \small Professor: G. Fiete}

\begin{document}

\maketitle

\begin{itemize}

  \item Associated Legendre Functions

    \begin{itemize}

      \item For $l=0,1,2,3\cdots$

        $$\left[(1-z^2)\frac{d^2}{dz^2}-2z\frac{d}{dz}+l(l+1)-\frac{m^2}{1-z^2}\right]P(z)0$$

      \item With:

        $$P_l^m(z)=P_l^{-m}(z)=(1-z^2)^{m/2}\frac{d^m}{dz^m}P_l(z)$$

      \item Since $P_l(z)$ is an $l$-th order polynomial, then $P_l^m(z)$ vanishes if $m>l$

      \item Properties of $P_l^m(z)$:

        \begin{itemize}

          \item $P_l^m(z)=0$ if $|m|>l$

          \item $P_l^m(z)=P_l^{-m}(z)$

          \item $P_l^m(\pm1)=0$ for $m\neq0$

          \item $P_l^m(-z)=(-1)^{l-m}P_l^{m}(z)$

          \item $\displaystyle \int_{-1}^1 P_l^m(z)P_q^m(z)\,dz=\frac{2}{2l+2}\cdot\frac{(l+m)!}{(l-m)!}\delta_{lq}$

        \end{itemize}

      \item We can obtain our $\Theta(\theta)$ function as:

        $$\Theta_l^m(\theta)=(-1)^m\frac{(2l+1)}{2}\frac{(l-m)!}{(l+m)!}P_l^k(\cos(\theta)),\quad m\geq0$$

        And:

        $$\Theta_l^{-m}(\theta)=(-1)^m\Theta_l^m(\theta)$$

      \item Here, we arrive at a point where the associated Legendre Functions are needed:

        $$P_o^o=1$$
        $$P_1^o=\cos(\theta)$$
        $$P_1^1=\sin(\theta)$$
        $$P_2^o=\frac{1}{2}(3\cos^3(\theta)-1)$$
        $$P_3^o=\frac{1}{2}(5\cos^5(\theta)-3\cos(\theta))$$

      \item Spherical Harmonics

        $$Y_l^m(\theta,\phi)=(-1)^{(m+|m|)/2}\sqrt{\frac{(2l+1)}{4\pi}\frac{(l-|m|)!}{(l+|m|)!}}P_l^m(\cos(\theta))e^{im\phi}$$
        $$Y_l^m(\theta,\phi)=(-1)(Y_l^m(\theta,\phi))^*$$

        Our first few values may be written as:

        $$Y_o^o(\theta,\phi)=\frac{1}{\sqrt{4\pi}}$$
        $$Y_1^o(\theta,\phi)=\sqrt{\frac{3}{4\pi}}\cos(\theta)$$
        $$Y_1^{\pm1}(\theta,\phi)=\mp\sqrt{\frac{3}{8\pi}}\sin(\theta)e^{\pm i\phi}$$

      \item Important Properties:

        \begin{itemize}

          \item Orthonormality:

            $$\bra{l_1m_1}\ket{l_2m_2}=\delta_{l_1l_2}\delta_{m_1m_2}$$

          \item Completeness:

            $$\psi(\theta,\phi)=\sum_{l=0}^{\infty}\sum_{m=-l}^l C_{lm}Y_l^m(\theta,\phi)$$
            $$C_{lm}=\bra{lm}\ket{\psi}=\int_0^{2\pi}\int_0^{\pi}(Y_l^m(\theta,\phi))^*\psi(\theta,\phi)\,d\Omega$$

          \item Parity:

            $$Y_l^m(\pi-\theta,\phi+\pi)=(-1)^lY_l^m(\theta,\phi)$$

        \end{itemize}

    \end{itemize}

\end{itemize}

\end{document}

